trillium/program_logic/int_ref.v
@@ -1,0 +1,47 @@
+From iris.proofmode Require Import tactics.
+From trillium.traces Require Export inftraces trace trace_utils.
+
+
+Section IntRef.
+  Context {St1 L1 St2 L2: Type}. 
+  Context (R: finite_trace St1 L1 -> finite_trace St2 L2 -> Prop). 
+  
+  (* TODO: find existing? *)
+  Definition int_ref_inf (tr1: trace St1 L1) (tr2: trace St2 L2) :=
+    forall i, R (trace_take_fwd i tr1) (trace_take_fwd i tr2).
+
+  Lemma int_ref_int_singleton (s1: St1) (s2: St2)
+    (REL0: R (trace_singleton s1) (trace_singleton s2)):
+    int_ref_inf ⟨ s1 ⟩ ⟨ s2 ⟩.
+  Proof using.
+    red. intros.
+    destruct i.
+    { done. }
+    do 2 (erewrite trace_take_fwd_short' with (i := S _) (j := 0); [| by rewrite from_trace_simpl| lia]). 
+    by rewrite !trace_take_fwd_0_first.
+  Qed.
+
+End IntRef.
+
+
+Section IntRefOne.
+  Context {St1 L1: Type}.
+  Context (R: finite_trace St1 L1 -> Prop). 
+
+  Definition int_ref_inf_one tr := forall i, R (trace_take_fwd i tr).
+
+
+End IntRefOne.
+
+
+Lemma int_ref_inf_impl {St1 L1 St2 L2}
+  (R Q: finite_trace St1 L1 -> finite_trace St2 L2 -> Prop)
+  (tr1: trace St1 L1) (tr2: trace St2 L2)
+  (IMPL: forall tr1 tr2, R tr1 tr2 -> Q tr1 tr2):
+  int_ref_inf R tr1 tr2 -> int_ref_inf Q tr1 tr2. 
+Proof using. intros ? ?. by apply IMPL. Qed. 
+
+Lemma int_ref_inf_proj_one {St1 L1 St2 L2} (R: finite_trace St1 L1 -> Prop)
+  (tr1: trace St1 L1) (tr2: trace St2 L2):
+  int_ref_inf (fun tr' _ => R tr') tr1 tr2 -> int_ref_inf_one R tr1.
+Proof using. done. Qed.
